examples/Toddler.v
@@ -1,0 +1,95 @@
+Require Import Bedrock.
+
+
+(** Always-0, in a convoluted way *)
+
+Definition always0S : assert := st ~> st#Rp @@ (st' ~> [| st'#Rv = $0 |]).
+
+Definition always0 := bmodule "always0" {{
+  bfunction "always0" [always0S] {
+    If (Rv = 0) {
+      Skip
+    } else {
+      Rv <- 0
+    };;
+    Goto Rp
+  }
+}}.
+
+Eval compute in compile always0.
+
+Theorem always0Ok : moduleOk always0.
+  structured; ho.
+Qed.
+
+
+(** Factorial! *)
+
+Lemma separated_0_4 : separated 0 4.
+  apply const_separated.
+(*  W_neq.
+Qed.*)
+Admitted.
+
+Lemma separated_4_0 : separated 4 0.
+(*  W_neq.
+Qed.*)
+Admitted.
+
+Hint Resolve separated_0_4 separated_4_0.
+
+Inductive factR : W -> W -> Prop :=
+| FR0 : factR 0 1
+| FRS : forall w r : W, w <> 0 -> factR (w ^- $1) r -> factR w (w ^* r).
+
+Lemma FR0' : forall w : W, w = 0 -> factR w 1.
+  intros; subst; apply FR0.
+Qed.
+
+Lemma FRS' : forall w r v : W, w <> 0 -> factR (w ^- $1) r -> v = w ^* r -> factR w v.
+  intros; subst; eapply FRS; eauto.
+Qed.
+
+Hint Resolve FR0' FRS'.
+
+Definition factS : assert := st ~> [| inBounds (fst st) 0 /\ inBounds (fst st) 4 |]
+  /\ st#Rp @@ (st' ~> [| factR st#Rv st'#Rv |]).
+
+Definition fact := bmodule "fact" {{
+  bfunction "fact" [factS] {
+    $[0] <- Rv;;
+    $[4] <- 1;;
+
+    [st ~> [| inBounds (fst st) 0 /\ inBounds (fst st) 4 |] /\ st#Rp @@ (st' ~> [| exists r, (factR st.[0] r /\ st'#Rv = st.[4] ^* r)%type |])]
+    While ($[0] <> 0) {
+      $[4] <- $[0] * $[4];;
+      $[0] <- $[0] - 1
+    };;
+
+    Rv <- $[4];;
+    Goto Rp
+  }
+}}.
+
+Eval compute in compile fact.
+
+Lemma times_1 : forall (n m x : W), factR n x
+  -> m = $1 ^* x
+  -> factR n m.
+  intros; subst; replace ($1 ^* x) with x by W_eq; auto.
+Qed.
+
+Hint Resolve times_1.
+
+Hint Extern 5 (@eq W ?X _) => match goal with
+                                | [ H : X = _ |- _ ] => rewrite H; clear H; W_eq
+                              end.
+
+Hint Extern 5 (@eq W _ _) => match goal with
+                               | [ |- ?G ] => has_evar G; fail 1
+                               | _ => W_eq
+                             end.
+
+Theorem factOk : moduleOk fact.
+  structured; (ho; eauto).
+Qed.
