src/Bedrock.v
@@ -1,4 +1,4 @@
-Require Export String List.
+Require Export String List NArith.
 
 Require Export Nomega Word IL LabelMap PropX PropXTac XCAP Structured StructuredModule Linker Programming.
 
